one-time pad is secure as per the one-time uniform ciphertext game

theories/examples/one_time_pad.v
@@ -1,4 +1,4 @@
-From clutch Require Export clutch lib.flip. 
+From clutch Require Export clutch lib.flip.
 Set Default Proof Using "Type*".
 
 Definition xor b1 b2 : expr :=
@@ -9,8 +9,11 @@ Definition xor_sem (b1 b2 : bool) :=
 
 Ltac foldxor := assert (forall b2, (if: _ then (if: b2 then #false else #true) else b2)%E = (xor _ _)) as -> by easy.
 
+(* The ideal encryption scheme returns a random bit. Can't get more uninformative than that.  *)
 Definition ideal : expr := λ:"msg", flip.
+(* The real one-time pad generates a random key the size of the message and returns the xor. *)
 Definition real : expr := λ:"msg", let: "k" := flip in xor "msg" "k".
+(* We want to show that "real" looks random, i.e. is indistinguishable from "ideal". *)
 
 Section logical_ref.
   Context `{!clutchRGS Σ}.
@@ -24,8 +27,11 @@ Section logical_ref.
   Global Instance xor_surj_1 : forall b, Surj (=) (xor_sem b) | 2.
   Proof. intros. apply cancel_surj. Qed.
 
-  Global Instance bij_xor : forall b, Bij (xor_sem b) | 2.
+  Global Instance xor_bij_1 : forall b, Bij (xor_sem b) | 2.
   Proof. constructor ; apply _. Qed.
+
+  Global Instance xor_comm : Comm (=) xor_sem | 2.
+  Proof. intros [] [] => //. Qed.
 
   Lemma xor_tp E (b1 b2 : bool) :
     ↑specN ⊆ E → ⊢ ∀ K, refines_right K (xor #b1 #b2) ={E}=∗ refines_right K (#(xor_sem b1 b2)).
@@ -34,7 +40,7 @@ Section logical_ref.
   Qed.
 
   Lemma xor_wp (b1 b2 : bool) :
-    ⊢ (WP xor #b1 #b2 {{v, ⌜v = #(xor_sem b1 b2)⌝}})%I.
+    ⊢ WP xor #b1 #b2 {{v, ⌜v = #(xor_sem b1 b2)⌝}}.
   Proof.
     rewrite /xor /xor_sem /negb. destruct b1, b2 ; wp_pures ; done.
   Qed.
@@ -45,18 +51,20 @@ Section logical_ref.
     rewrite /xor /xor_sem /negb. destruct b1, b2 ; rel_pures_l ; rel_values ; done.
   Qed.
 
+  (* We should a bi-refinement, carefully choosing the relation of the sampled bits. *)
   Lemma real_ideal_rel :
     ⊢ REL real << ideal : lrel_bool → lrel_bool.
-  Proof.
+  Proof with foldxor.
+    rewrite /real /ideal.
     rel_arrow_val.
     iIntros (msg1 msg2) "Hmsg".
     rel_pures_l. rel_pures_r.
     foldxor.
-    iDestruct "Hmsg" as "[%b [-> ->]]".
-    rel_apply (refines_couple_flip_flip (xor_sem b)).
+    iDestruct "Hmsg" as "[%b_msg [-> ->]]".
+    rel_apply (refines_couple_flip_flip (xor_sem b_msg)).
+    simpl.
     iIntros (k).
-    rel_pures_l.
-    foldxor.
+    rel_pures_l...
     iApply xor_xor_sem.
   Qed.
 
@@ -73,6 +81,77 @@ Section logical_ref.
     rel_pures_r.
     foldxor.
     unshelve rel_apply_r (refines_steps_r $! (xor_tp _ _ _ _)) ; [easy|].
+    rewrite cancel.
+    rel_values.
+  Qed.
+
+  (* We prove that the OTP has "one-time uniform ciphertexts". *)
+  Definition L_ots_rand_real (size keygen enc : expr) : expr :=
+    λ: "m" ,
+      let: "k" := keygen #() in
+      enc "k" "m".
+
+  Definition sampler : expr :=
+    rec: "f" "n" :=
+      if: "n" < #1 then
+        #()
+      else
+        let: "b" := flip in
+        ("b", "f" ("n" - #1)).
+
+  Definition L_ots_rand_rand (size keygen enc : expr) : expr :=
+    λ: "_" ,
+      sampler size.
+
+  Definition keygen := (λ:<>, flip)%E.
+  Definition enc := (λ:"k" "m", (xor "k" "m", #()))%E.
+  Definition size := 1.
+
+  Fixpoint lrel_bitlist n : lrel Σ :=
+    match n with
+    | O => lrel_unit
+    | S n' => lrel_prod lrel_bool (lrel_bitlist n')
+    end.
+
+  Lemma L_ots_rr :
+    ⊢ REL L_ots_rand_real #size keygen enc
+      << L_ots_rand_rand #size keygen enc
+      : lrel_bool → lrel_bitlist size.
+  Proof.
+    unfold L_ots_rand_rand, L_ots_rand_real, enc, keygen.
+    rel_arrow_val.
+    iIntros (msg1 msg2) "[%msg [-> ->]]" ;
+      rel_pures_l ; rel_pures_r.
+    rel_apply (refines_couple_flips (xor_sem msg)) => /=.
+    iIntros (k).
+    rel_pures_l.
+    foldxor.
+    do 6 rel_pure_r.
+    iApply refines_pair.
+    2: rel_values.
+    rewrite /xor /xor_sem /negb.
+    destruct k, msg ; rel_pures_l ; rel_values ; done.
+  Qed.
+
+  Lemma L_ots_rr' :
+    ⊢ REL L_ots_rand_rand #size keygen enc
+      << L_ots_rand_real #size keygen enc
+      : lrel_bool → lrel_bitlist size.
+  Proof.
+    unfold L_ots_rand_rand, L_ots_rand_real, enc, keygen.
+    rel_arrow_val.
+    iIntros (msg1 msg2) "[%msg [-> ->]]" ;
+      rel_pures_l ; rel_pures_r.
+    rel_apply (refines_couple_flips (xor_sem msg)) => /=.
+    iIntros (k).
+    do 6 rel_pure_l.
+    rel_pures_r.
+    foldxor.
+    unshelve rel_apply_r (refines_steps_r $! (xor_tp _ _ _ _)) ; [easy|].
+    iModIntro.
+    iApply refines_pair.
+    2: rel_values.
+    rewrite comm.
     rewrite cancel.
     rel_values.
   Qed.
